feat: Array lemma alignment; fold and map (#6546)
This PR continues aligning `Array` and `Vector` lemmas with `List`,
working on `fold` and `map` operations.

src/Init/Data/Vector/Basic.lean
@@ -136,6 +136,18 @@ This will perform the update destructively provided that the vector has a refere
 @[inline] def set! (v : Vector α n) (i : Nat) (x : α) : Vector α n :=
   ⟨v.toArray.set! i x, by simp⟩
 
+@[inline] def foldlM [Monad m] (f : β → α → m β) (b : β) (v : Vector α n) : m β :=
+  v.toArray.foldlM f b
+
+@[inline] def foldrM [Monad m] (f : α → β → m β) (b : β) (v : Vector α n) : m β :=
+  v.toArray.foldrM f b
+
+@[inline] def foldl (f : β → α → β) (b : β) (v : Vector α n) : β :=
+  v.toArray.foldl f b
+
+@[inline] def foldr (f : α → β → β) (b : β) (v : Vector α n) : β :=
+  v.toArray.foldr f b
+
 /-- Append two vectors. -/
 @[inline] def append (v : Vector α n) (w : Vector α m) : Vector α (n + m) :=
   ⟨v.toArray ++ w.toArray, by simp⟩
